Move diskSizes into Coq and give it a spec
Might not do exactly the same thing when files are missing (haven't
really tested error cases recently), but we can potentially figure out
how to put in some error handling. The main concern would be both disks
failing (that is, running the server without either disk image), which
the Coq proofs forbid using the dependently typed proof inside two disk
states.

replicate-nbd/src/Network/NBD.hs
@@ -16,7 +16,6 @@ import           Interface (InitResult(..))
 import NbdData
 import           Network.NBD.Data
 import           Replication.TwoDiskEnvironment
-import           Replication.TwoDiskOps
 import qualified Server
 import           System.Exit (die)
 import           Utils.Conversion
@@ -175,12 +174,12 @@ forkNbdServer e doLog =
       name <- negotiateNewstyle
       liftIO $ when (name /= "") $
         putStrLn $ "ignoring non-default export name " ++ show name
-      msz <- liftIO . runTD e $ diskSizes
+      msz <- liftIO . runTD e $ Server.diskSizes
       case msz of
         Left (sz0, sz1) -> throwM $ SizeMismatchException sz0 sz1
         Right sz ->
           -- start transmission phase
-          sendExportInformation (fromIntegral sz)
+          sendExportInformation (fromIntegral sz * blocksize)
       liftIO $ putStrLn "negotiated with client"
       -- infinite loop parsing commands and putting them on the queue
       handleCommands doLog e
