src/SeqDisk/ArrayAPI.v
@@ -27,12 +27,6 @@ Section ArrayDisk.
       apply (write (off+1) _ rest).
   Defined.
 
-  (* For the convenience of the extracted Haskell code we define short functions
-     to access the final implementation. *)
-
-  Definition diskSize : prog nat :=
-    Prim d D.DiskSize.
-
   Definition recover : prog unit :=
     irec d.
 
